Proved a lot of things about Binomial Heaps. Defined physicist's queues as in chapter 6.4.2 of Okasaki and proved that snoc and tail preserve the property of being a valid queue. Defined Sortable collections as in chapter 6.4.3 of Okasaki, but didn't prove anything interesting.

DS/BinomialHeap.v
@@ -8,7 +8,36 @@ Inductive Tree (A : Type) : Type :=
 
 Arguments T [A] _ _ _.
 
+Inductive elemTree {A : Type} (x : A) : Tree A -> Prop :=
+    | elemTree_root :
+        forall (n : nat) (l : list (Tree A)), elemTree x (T n x l)
+    | elemTree_child :
+        forall (n : nat) (y : A) (l : list (Tree A)) (t : Tree A),
+          elemTree x t -> In t l -> elemTree x (T n y l).
+
+Hint Constructors elemTree.
+
 Definition Heap (A : Type) : Type := list (Tree A).
+
+Definition elem {A : Type} (x : A) (h : Heap A) : Prop :=
+  exists t : Tree A, elemTree x t /\ In t h.
+
+Inductive elemTree' {A : Type} (x : A) : Tree A -> Prop :=
+    | elemTree'_root :
+        forall (n : nat) (l : list (Tree A)), elemTree' x (T n x l)
+    | elemTree'_heap :
+        forall h : Heap A, elemHeap x h ->
+          forall (n : nat) (y : A), elemTree' x (T n y h)
+
+with elemHeap {A : Type} (x : A) : Heap A -> Prop :=
+    | elemHeap_here :
+        forall (t : Tree A) (h' : Heap A),
+          elemTree' x t -> elemHeap x (t :: h')
+    | elemHeap_there :
+        forall (t : Tree A) (h' : Heap A),
+          elemHeap x h' -> elemHeap x (t :: h').
+
+Hint Constructors elemTree' elemHeap.
 
 Definition empty {A : Type} : Heap A := [].
 
@@ -67,38 +96,7 @@ match h1 with
         in aux h2
 end.
 
-(*Fixpoint merge {A : LinDec} (h1 h2 : Heap A) : Heap A :=
-match h1, h2 with
-    | [], _ => h2
-    | _, [] => h1
-    | t1 :: h1', t2 :: h2' =>
-        if rank t1 <? rank t2
-        then t1 :: merge h1' h2
-        else
-          if rank t2 <? rank t1
-          then t2 :: merge h1 h2'
-          else insTree (link t1 t2) (merge h1' h2')
-end.*)
-
-Lemma merge_spec :
-  forall (A : LinDec) (h1 h2 : Heap A),
-    merge h1 h2 =
-    match h1, h2 with
-        | [], _ => h2
-        | _, [] => h1
-        | t1 :: h1', t2 :: h2' =>
-            if rank t1 <? rank t2
-            then t1 :: merge h1' h2
-            else
-              if rank t2 <? rank t1
-              then t2 :: merge h1 h2'
-              else insTree (link t1 t2) (merge h1' h2')
-    end.
-Proof.
-  destruct h1, h2; reflexivity.
-Qed.
-
-Fixpoint removeMinTree
+Function removeMinTree
   {A : LinDec} (h : Heap A) : option (Tree A * Heap A) :=
 match h with
     | [] => None
@@ -125,4 +123,378 @@ match removeMinTree h with
     | Some (T _ x h1, h2) => Some (merge h1 h2)
 end.
 
-Import PriorityQueue.
+Definition unMin {A : LinDec} (h : Heap A) : option (A * Heap A) :=
+match removeMinTree h with
+    | None => None
+    | Some (T _ x h1, h2) => Some (x, merge h1 h2)
+end.
+
+(** spec of merge *)
+
+Lemma merge_spec :
+  forall (A : LinDec) (h1 h2 : Heap A),
+    merge h1 h2 =
+    match h1, h2 with
+        | [], _ => h2
+        | _, [] => h1
+        | t1 :: h1', t2 :: h2' =>
+            if rank t1 <? rank t2
+            then t1 :: merge h1' h2
+            else
+              if rank t2 <? rank t1
+              then t2 :: merge h1 h2'
+              else insTree (link t1 t2) (merge h1' h2')
+    end.
+Proof.
+  destruct h1, h2; reflexivity.
+Qed.
+
+(** Properties of [isEmpty]. *)
+
+Lemma isEmpty_elem :
+  forall (A : LinDec) (h : Heap A),
+    isEmpty h = true <-> forall x : A, ~ elem x h.
+Proof.
+  split; intro.
+    inv 1. inv H1. destruct h; cbn in *.
+      assumption.
+      congruence.
+    induction h; intros.
+      reflexivity.
+      destruct h; cbn in *.
+        destruct a. specialize (H c). contradict H.
+          red. exists (T n c l). split; cbn; auto.
+        apply IHh. do 2 intro. apply (H x). red. inv H0. inv H1.
+          exists x0. cbn. auto.
+Qed.
+
+Lemma isEmpty_elemHeap :
+  forall (A : LinDec) (h : Heap A),
+    isEmpty h = true <-> forall x : A, ~ elemHeap x h.
+Proof.
+  split; intro.
+    inv 1; cbn in *; congruence.
+    induction h; intros.
+      cbn. reflexivity.
+      specialize (H (root a)). contradiction H. destruct a. cbn.
+        apply elemHeap_here. auto.
+Qed.
+
+Lemma isEmpty_empty_false :
+  forall {A : LinDec} (h : Heap A),
+    isEmpty h = false <-> h <> empty.
+Proof.
+  destruct h; compute; firstorder congruence.
+Qed.
+
+Lemma isEmpty_empty_true :
+  forall (A : LinDec) (h : Heap A),
+    isEmpty h = true <-> h = empty.
+Proof.
+  destruct h; compute; firstorder congruence.
+Qed.
+
+Lemma isEmpty_insTree :
+  forall (A : LinDec) (t : Tree A) (h : Heap A),
+    isEmpty (insTree t h) = false.
+Proof.
+  intros A t h; gen t.
+  induction h as [| t' h']; cbn; intros.
+    reflexivity.
+    destruct t'; cbn. destruct n as [| n'].
+      apply IHh'.
+      destruct t. cbn. destruct (leb n n').
+        cbn. reflexivity.
+        apply IHh'.
+Qed.
+
+Lemma isEmpty_insert :
+  forall {A : LinDec} (x : A) (h : Heap A),
+    isEmpty (insert x h) = false.
+Proof.
+  intros. unfold insert. apply isEmpty_insTree.
+Qed.
+
+Lemma isEmpty_merge :
+  forall {A : LinDec} (h1 h2 : Heap A),
+    isEmpty (merge h1 h2) = isEmpty h1 && isEmpty h2.
+Proof.
+  destruct h1, h2; rewrite merge_spec; cbn; auto.
+  repeat match goal with
+      | |- context [if ?x then _ else _] => destruct x
+  end; cbn.
+    1-2: reflexivity.
+    rewrite isEmpty_insTree. reflexivity.
+Qed.
+
+Lemma isEmpty_removeMinTree_false :
+  forall (A : LinDec) (t : Tree A) (h h' : Heap A),
+    removeMinTree h = Some (t, h') -> isEmpty h = false.
+Proof.
+  intros. destruct h; cbn in *; congruence.
+Qed.
+
+Lemma isEmpty_removeMinTree_false' :
+  forall (A : LinDec) (h : Heap A),
+    isEmpty h = false <->
+    exists (t : Tree A) (h' : Heap A), removeMinTree h = Some (t, h').
+Proof.
+  split.
+    functional induction @removeMinTree A h; cbn; intros; eauto.
+      congruence.
+      rewrite e0 in IHo. destruct h'; cbn in *.
+        contradiction.
+        apply IHo. reflexivity.
+    destruct 1 as [t [h' H]]. destruct h; cbn in *; congruence.
+Qed.
+
+Lemma isEmpty_removeMinTree_true :
+  forall (A : LinDec) (h : Heap A),
+    removeMinTree h = None <-> isEmpty h = true.
+Proof.
+  split.
+    functional induction @removeMinTree A h; cbn; try congruence.
+      destruct h'; auto.
+    destruct h; cbn; congruence.
+Qed.
+
+Lemma isEmpty_unMin_false :
+  forall (A : LinDec) (h : Heap A),
+    isEmpty h = false <->
+    exists (m : A) (h' : Heap A), unMin h = Some (m, h').
+Proof.
+  split; unfold unMin; intros.
+    apply isEmpty_removeMinTree_false' in H. destruct H as [t [h' H]].
+      destruct t as [r x h'']. exists x, (merge h'' h'). rewrite H. auto.
+    destruct H as [m [h' H]]. apply isEmpty_removeMinTree_false'.
+      case_eq (removeMinTree h); intros.
+        destruct p. eauto.
+        rewrite H0 in H. congruence.
+Qed.
+
+Lemma isEmpty_unMin_true :
+  forall (A : LinDec) (h : Heap A),
+    isEmpty h = true <-> unMin h = None.
+Proof.
+  unfold unMin; split; intros.
+    apply isEmpty_removeMinTree_true in H. rewrite H. reflexivity.
+    case_eq (removeMinTree h); intros.
+      rewrite H0 in H. destruct p, t. inv H.
+      apply isEmpty_removeMinTree_true. assumption.
+Qed.
+
+(** Properties of [link]. *)
+
+Lemma link_elemTree :
+  forall (A : LinDec) (x : A) (t1 t2 : Tree A),
+    elemTree x (link t1 t2) <-> elemTree x t1 \/ elemTree x t2.
+Proof.
+  split.
+    destruct t1, t2; cbn; intro; dec.
+      inv H. inv H4. eauto.
+      inv H. inv H4. eauto.
+    inv 1.
+      destruct t1, t2; cbn; dec.
+        inv H0. eapply elemTree_child; cbn; eauto.
+        inv H0.
+          eapply elemTree_child; cbn; eauto.
+          eapply elemTree_child.
+            exact H2.
+            cbn.
+
+Abort.
+
+Ltac tree :=
+repeat match goal with
+    | H : context [if ?x then _ else _] |- _ => destruct x
+    | |- context [if ?x then _ else _] => destruct x
+end; auto.
+
+Ltac tree' := intros; cbn in *;
+repeat match goal with
+    | H : context [if ?x then _ else _] |- _ => destruct x
+    | |- context [if ?x then _ else _] => destruct x
+    | H : _ \/ _ |- _ => inv H
+    | H : elemTree' _ (T _ _ _) |- _ => inv H
+    | H : elemHeap _ [] |- _ => inv H
+    | H : elemHeap _ (_ :: _) |- _ => inv H
+end; auto.
+
+Lemma link_elemTree' :
+  forall (A : LinDec) (x : A) (t1 t2 : Tree A),
+    elemTree' x (link t1 t2) <-> elemTree' x t1 \/ elemTree' x t2.
+Proof.
+  split; destruct t1, t2; cbn; intros; dec; tree'.
+Qed.
+
+Hint Extern 0 =>
+match goal with
+    | |- context [elemTree' _ (link _ _)] =>
+        rewrite link_elemTree'
+end.
+
+Lemma insTree_elemHeap :
+  forall (A : LinDec) (x : A) (t : Tree A) (h : Heap A),
+    elemHeap x (insTree t h) <-> elemTree' x t \/ elemHeap x h.
+Proof.
+  split.
+    gen t; gen x. induction h as [| t' h']; tree'.
+      specialize (IHh' _ _ H). rewrite link_elemTree' in IHh'.
+        firstorder.
+    gen t; gen x. induction h as [| t' h']; tree'.
+Restart.
+  split; gen t; gen x; induction h as [| t' h']; tree'.
+  specialize (IHh' _ _ H). rewrite link_elemTree' in IHh'. firstorder.
+Qed.
+
+Lemma insert_elemTree' :
+  forall (A : LinDec) (x : A) (h : Heap A),
+    elemHeap x (insert x h).
+Proof.
+  intros. unfold insert. rewrite insTree_elemHeap. auto.
+Qed.
+
+Lemma merge_elemHeap :
+  forall (A : LinDec) (x : A) (h1 h2 : Heap A),
+    elemHeap x (merge h1 h2) <-> elemHeap x h1 \/ elemHeap x h2.
+Proof.
+  split; gen h2.
+    induction h1.
+      cbn. auto.
+      intros. induction h2.
+        auto.
+        cbn in H. tree'.
+          specialize (IHh1 _ H1). firstorder.
+          Focus 2. rewrite insTree_elemHeap, link_elemTree' in H.
+            decompose [or] H; clear H; auto. specialize (IHh1 _ H0). inv IHh1.
+          specialize (IHh2 H1). inv IHh2.
+Restart.
+  split; gen h2.
+    induction h1; induction h2; tree'.
+      specialize (IHh1 _ H1). firstorder.
+      specialize (IHh2 H1). inv IHh2.
+      clear IHh2. rewrite insTree_elemHeap, link_elemTree' in H.
+        decompose [or] H; clear H; auto. specialize (IHh1 _ H0). inv IHh1.
+    induction h1; induction h2; tree';
+      rewrite insTree_elemHeap, link_elemTree'; auto.
+Qed.
+
+Lemma removeMinTree_elemHeap :
+  forall (A : LinDec) (x : A) (t : Tree A) (h h' : Heap A),
+    removeMinTree h = Some (t, h') ->
+      elemHeap x h <-> elemTree' x t \/ elemHeap x h'.
+Proof.
+  split.
+    functional induction @removeMinTree A h; inv 1; inv H.
+      specialize (IHo x _ _ e0 H2). inv IHo.
+    functional induction @removeMinTree A h; inv 1; inv H.
+      specialize (IHo x _ _ e0 ltac:(auto)). inv IHo.
+      inv H1. specialize (IHo x _ _ e0 ltac:(auto)). inv IHo.
+Qed.
+
+Lemma unMin_elemHeap :
+  forall (A : LinDec) (x m : A) (h h' : Heap A),
+    unMin h = Some (m, h') ->
+      elemHeap x h <-> x = m \/ elemHeap x h'.
+Proof.
+  unfold unMin. split.
+    case_eq (removeMinTree h); intros; rewrite H0 in *.
+      destruct p, t. inv H.
+        apply removeMinTree_elemHeap with (x := x) in H0.
+        rewrite merge_elemHeap. firstorder. inv H.
+      congruence.
+    case_eq (removeMinTree h); intros; rewrite H0 in *.
+      destruct p, t. inv H. rewrite merge_elemHeap in *.
+        apply removeMinTree_elemHeap with (x := x) in H0.
+        firstorder; subst; auto.
+      congruence.
+Qed.
+
+Lemma removeMinTree_insTree :
+  forall (A : LinDec) (t : Tree A) (h : Heap A),
+    removeMinTree (insTree t h) <> None.
+Proof.
+  repeat intro. apply isEmpty_removeMinTree_true in H.
+  rewrite isEmpty_insTree in H. congruence.
+Qed.
+
+Lemma unMin_insTree :
+  forall (A : LinDec) (t : Tree A) (h : Heap A),
+    unMin (insTree t h) <> None.
+Proof.
+  intros. unfold unMin.
+  case_eq (removeMinTree (insTree t h)); intros.
+    destruct p, t0. inv 1.
+    apply removeMinTree_insTree in H. contradiction.
+Qed.
+
+Lemma unMin_insert :
+  forall (A : LinDec) (x : A) (h : Heap A),
+    unMin (insert x h) <> None.
+Proof.
+  intros. unfold insert. apply unMin_insTree.
+Qed.
+
+Lemma unMin_merge :
+  forall (A : LinDec) (h1 h2 : Heap A),
+    unMin (merge h1 h2) = None <->
+    unMin h1 = None /\ unMin h2 = None.
+Proof.
+  intros. rewrite <- !isEmpty_unMin_true, isEmpty_merge.
+  destruct h1, h2; cbn; firstorder congruence.
+Qed.
+
+(** Counting shiet. *)
+
+Fixpoint count_Tree {A : LinDec} (x : A) (t : Tree A) : nat :=
+match t with
+    | T _ x' l =>
+        (if x =? x' then S else id)
+          (fold_right (fun t ts => count_Tree x t + ts) 0 l)
+end.
+
+Definition count_Heap {A : LinDec} (x : A) (h : Heap A) : nat :=
+  fold_right (fun t ts => count_Tree x t + ts) 0 h.
+
+Lemma isEmpty_count_Tree :
+  forall (A : LinDec) (t : Tree A),
+    isEmpty [t] = true <-> forall x : A, count_Tree x t = 0.
+Proof.
+  split; cbn; intros.
+    congruence.
+    specialize (H (root t)). destruct t. cbn in H. dec.
+Qed.
+
+Lemma count_Tree_link :
+  forall (A : LinDec) (x : A) (t1 t2 : Tree A),
+    count_Tree x (link t1 t2) = count_Tree x t1 + count_Tree x t2.
+Proof.
+  destruct t1, t2. cbn. do 2 dec; unfold id; omega.
+Qed.
+
+Lemma insTree_Some :
+  forall (A : LinDec) (t : Tree A) (h : Heap A),
+    exists (t' : Tree A) (h' : Heap A),
+      insTree t h = t' :: h'.
+Proof.
+  intros A t h; gen t. induction h as [| t' h']; tree'; eauto.
+Qed.
+
+Lemma count_Heap_insTree :
+  forall (A : LinDec) (x : A) (t : Tree A) (h : Heap A),
+    count_Heap x (insTree t h) = count_Tree x t + count_Heap x h.
+Proof.
+  intros A x t h; gen t; gen x.
+  induction h as [| t' h']; cbn; intros.
+    reflexivity.
+    tree'. unfold count_Heap in *. rewrite IHh'.
+      rewrite count_Tree_link. omega.
+Qed.
+
+Lemma count_Heap_insert :
+  forall (A : LinDec) (x y : A) (h : Heap A),
+    count_Heap x (insert y h) =
+    (if x =? y then S else id) (count_Heap x h).
+Proof.
+  intros. unfold insert. rewrite count_Heap_insTree. cbn. dec.
+Qed.
