ADT/Sortable.v
@@ -1,0 +1,133 @@
+Add Rec LoadPath "/home/zeimer/Code/Coq".
+
+Require Import RCCBase.
+Require Import Structures.LinDec.
+Require Import Sorting.Sort.
+
+Require Import HSLib.Instances.Lazy.
+
+(** Sortable collections as in chapter 6.4.3 of Okasaki. *)
+
+Module Type Sortable.
+
+Parameter Sortable : LinDec -> Type.
+
+Parameter empty :
+  forall {A : LinDec}, Sortable A.
+
+Parameter add :
+  forall {A : LinDec}, A -> Sortable A -> Sortable A.
+
+Parameter sort :
+  forall {A : LinDec}, Sortable A -> list A.
+
+Parameter sort_sorted :
+  forall {A : LinDec} (s : Sortable A),
+    sorted A (sort s).
+
+End Sortable.
+
+Module Sortable_BottomUpMergesortWithSharing.
+
+Definition Sortable (A : LinDec) : Type :=
+  nat * Lazy (list (list A)).
+
+Definition empty {A : LinDec} : Sortable A :=
+  (0, delay []).
+
+Require Import Div2.
+
+Function isEven (n : nat) : bool :=
+match n with
+    | 0 => true
+    | 1 => false
+    | S (S n') => isEven n'
+end.
+
+Fixpoint merge {A : LinDec} (l1 l2 : list A) : list A :=
+match l1 with
+    | [] => l2
+    | h1 :: t1 =>
+        let
+          aux := fix aux (l1 l2 : list A) : list A :=
+          match l2 with
+              | [] => l1
+              | h2 :: t2 =>
+                  if h1 <=? h2
+                  then h1 :: merge t1 l2
+                  else h2 :: aux l1 t2
+          end
+        in aux l1 l2
+end.
+
+Fixpoint addSeg_aux
+  {A : LinDec} (seg : list A) (segs : list (list A)) (size : nat)
+  : list (list A) :=
+match segs with
+    | [] => [seg]
+    | seg' :: segs' =>
+        if isEven size
+        then seg :: segs
+        else addSeg_aux (merge seg seg') segs' (div2 size)
+end.
+
+Definition addSeg
+  {A : LinDec} (x : A) (s : Sortable A) : Sortable A :=
+    let '(size, segs) := s in
+      (1 + size, delay (addSeg_aux [x] (force segs) size)).
+
+Fixpoint sort_aux
+  {A : LinDec} (seg : list A) (segs : list (list A)) : list A :=
+match segs with
+    | [] => seg
+    | seg' :: segs' => sort_aux (merge seg seg') segs'
+end.
+
+Fixpoint sort {A : LinDec} (s : Sortable A) : list A :=
+  let '(_, segs) := s in sort_aux [] (force segs).
+
+Lemma addSeg_aux_not_nil :
+  forall (A : LinDec) (seg : list A) (segs : list (list A)) (size : nat),
+    addSeg_aux seg segs size <> [].
+Proof.
+  intros A seg segs size; gen size; gen seg.
+  induction segs as [| seg' segs']; cbn; intros.
+    inv 1.
+    destruct (isEven size).
+      inv 1.
+      apply IHsegs'.
+Qed.
+
+Lemma merge_eq :
+  forall (A : LinDec) (l1 l2 : list A),
+    merge l1 l2 =
+    match l1, l2 with
+        | [], _ => l2
+        | _, [] => l1
+        | h1 :: t1, h2 :: t2 =>
+            if h1 <=? h2
+            then h1 :: merge t1 l2
+            else h2 :: merge l1 t2
+    end.
+Proof.
+  destruct l1, l2; reflexivity.
+Qed.
+
+Lemma merge_sorted :
+  forall (A : LinDec) (l1 l2 : list A),
+    sorted A l1 -> sorted A l2 -> sorted A (merge l1 l2).
+Proof.
+  induction 1; intros.
+    cbn. assumption.
+    induction H.
+      cbn. dec.
+      cbn. dec.
+      rewrite !merge_eq.
+Restart.
+  induction l1 as [| h1 t1]; induction l2 as [| h2 t2]; intros.
+    1-3: assumption.
+    rewrite merge_eq. dec.
+      case_eq (merge t1 (h2 :: t2)); intros; auto.
+Abort.
+
+Require Import Sorting.MergeSort.
