DS/PhysicistsQueue.v
@@ -1,0 +1,175 @@
+Add Rec LoadPath "/home/zeimer/Code/Coq".
+
+Require Import RCCBase.
+
+Require Import HSLib.Instances.Lazy.
+
+Require Import Structures.LinDec.
+
+Definition Queue (A : Type) : Type :=
+  list A * nat * Lazy (list A) * nat * list A.
+
+Definition empty {A : Type} : Queue A :=
+  ([], 0, delay [], 0, []).
+
+Definition isEmpty {A : Type} (q : Queue A) : bool :=
+  let '(w, _, _, _, _) := q in
+match w with
+    | [] => true
+    | _ => false
+end.
+
+Definition checkw {A : Type} (q : Queue A) : Queue A :=
+  let '(w, lenf, f, lenr, r) := q in
+match w with
+    | [] => (force f, lenf, f, lenr, r)
+    | _ => q
+end.
+
+Definition queue {A : Type} (q : Queue A) : Queue A :=
+  let '(w, lenf, f, lenr, r) := q in
+  if @leqb natle lenr lenf
+  then checkw q
+  else
+    let
+      f' := force f
+    in
+      checkw (f', lenf + lenr, delay (force f ++ rev r), 0, []).
+
+Print queue.
+
+Definition snoc {A : Type} (x : A) (q : Queue A) : Queue A :=
+  let '(w, lenf, f, lenr, r) := q in
+    queue (w, lenf, f, 1 + lenr, x :: r).
+
+Definition tl {A : Type} (l : list A) : list A :=
+match l with
+    | [] => []
+    | _ :: t => t
+end.
+
+Definition tail {A : Type} (q : Queue A) : option (Queue A) :=
+  let '(w, lenf, f, lenr, r) := q in
+match w with
+    | [] => None
+    | h :: t => Some (queue (t, pred lenf, delay (tl (force f)), lenr, r))
+end.
+
+Definition head {A : Type} (q : Queue A) : option A :=
+  let '(w, lenf, f, lenr, r) := q in
+match w with
+    | [] => None
+    | h :: _ => Some h
+end.
+
+(** The queue invariant. *)
+
+Inductive prefix {A : Type} : list A -> list A -> Prop :=
+    | prefix_nil :
+        forall l : list A, prefix [] l
+    | prefix_cons :
+        forall (h : A) (t l : list A),
+          prefix t l -> prefix (h :: t) (h :: l).
+
+Hint Constructors prefix.
+
+Lemma prefix_app :
+  forall (A : Type) (l1 l2 : list A),
+    prefix l1 (l1 ++ l2).
+Proof.
+  induction l1 as [| h1 t1]; cbn; auto.
+Qed.
+
+Lemma prefix_refl :
+  forall (A : Type) (l : list A),
+    prefix l l.
+Proof.
+  induction l; auto.
+Qed.
+
+Hint Resolve prefix_app prefix_refl.
+
+Lemma prefix_char :
+  forall (A : Type) (l1 l2 : list A),
+    prefix l1 l2 <-> exists suffix : list A, l1 ++ suffix = l2.
+Proof.
+  split.
+    induction 1; cbn; firstorder eauto. exists x. congruence.
+    destruct 1 as [suffix <-]. apply prefix_app.
+Qed.
+
+Definition isQueue {A : Type} (q : Queue A) : Prop :=
+  let '(w, lenf, f, lenr, r) := q in
+    prefix w (force f) /\ lenf = length (force f)
+    /\ lenr = length r /\ lenr <= lenf.
+
+Lemma empty_isQueue :
+  forall A : Type, isQueue (@empty A).
+Proof. cbn. auto. Qed.
+
+Ltac q := repeat
+match goal with
+    | |- forall q : Queue _, _ =>
+        let w := fresh "w" in
+        let lenf := fresh "lenf" in
+        let f := fresh "f" in
+        let lenr := fresh "lenr" in
+        let r := fresh "r" in
+          destruct q as [[[[w lenf] f] lenr] r]
+    | |- forall _, _ => intro
+end.
+
+Lemma queue_isQueue :
+  forall (A : Type) (q : Queue A),
+    isQueue (queue q).
+Proof.
+  q. cbn. case_eq (Nat.leb lenr lenf); intros.
+    destruct w. cbn. firstorder.
+      cbn.
+Abort.
+
+Lemma checkw_isQueue :
+  forall (A : Type) (q : Queue A),
+    isQueue (checkw q).
+Proof.
+  q. cbn. destruct w. cbn.
+Abort.
+
+Lemma snoc_isQueue :
+  forall (A : Type) (x : A) (q : Queue A),
+    isQueue q -> isQueue (snoc x q).
+Proof.
+  q. cbn in *. destruct lenf as [| lenf']; cbn.
+    firstorder. destruct (force f); cbn in *; try congruence.
+      firstorder. rewrite app_length. cbn. rewrite rev_length. omega.
+    firstorder. case_eq (leb lenr lenf'); intros.
+      apply leb_complete in H3. destruct w; cbn; firstorder.
+      destruct (force f); cbn in *; firstorder.
+        rewrite !app_length, rev_length. cbn. omega.
+Qed.
+
+Lemma force_delay :
+  forall (A : Type) (x : A),
+    force (delay x) = x.
+Proof. compute. reflexivity. Qed.
+
+Lemma tail_isQueue :
+  forall (A : Type) (q q' : Queue A),
+    tail q = Some q' -> isQueue q -> isQueue q'.
+Proof.
+  q; cbn in *. destruct w.
+    inv H.
+    case_eq (leb lenr (pred lenf)); intro; rewrite H1 in *.
+      destruct w; inv H; rewrite force_delay; firstorder.
+        destruct (force f); cbn in *; subst; auto.
+        apply leb_complete in H1. auto.
+        inv H.
+        inv H. rewrite <- H7. cbn. reflexivity.
+        apply leb_complete in H1. auto.
+      rewrite !force_delay in *. destruct (force f); cbn in *; inv H.
+        firstorder. rewrite force_delay, rev_length.
+          apply leb_complete_conv in H1. omega.
+        destruct l; inv H3; firstorder; rewrite force_delay; inv H.
+          rewrite rev_length. cbn. reflexivity.
+          cbn. rewrite app_length, rev_length. reflexivity.
+Qed.
